Env: Use weak rather than ordered sets
'Weak' in this case simply means that the sets only require a decidable
equality over the underlying type, not an ordering. Since we don't care
about the efficiency of our sets anyway, this makes no difference to us,
and dropping the ordering means less busywork.

src/Var.v
@@ -66,55 +66,9 @@ Hint Resolve beq_nat_sym : env.
 Lemma beq_var_sym : forall x y, beq_var x y = beq_var y x.
 Proof. intros. destruct x; destruct y; unfold beq_var. apply beq_nat_sym. Qed.
 
-Module VarOrder <: OrderedType.
-
-  Module N := PeanoNat.Nat.
-  Module NF := OrderedTypeFacts N.
-
+Module VarEq <: DecidableType.
   Definition t := Var.
   Definition eq (x y : Var) := eq x y.
-  Definition lt (x y : Var) :=
-    match x, y with
-    | mkVar n, mkVar m => lt n m
-    end
-  .
-  Definition compare (x y : Var) :=
-    match x, y with
-    | mkVar n, mkVar m => N.compare n m
-    end
-  .
-
-  Definition eq_equiv := eq_equivalence (A := Var).
+  Instance eq_equiv : Equivalence eq := @eq_equivalence Var.
   Definition eq_dec := eq_Var_dec.
-
-  Instance lt_irreflexive : Irreflexive lt.
-  Proof.
-    unfold Irreflexive. unfold Reflexive. unfold complement. intros x H.
-    destruct x. unfold lt in H. apply StrictOrder_Irreflexive in H. assumption.
-  Qed.
-
-  Instance lt_transitive : Transitive lt.
-  Proof.
-    unfold Transitive. intros x y z Hxy Hyz. destruct x; destruct y; destruct z.
-    unfold lt in *. eapply transitivity; eassumption.
-  Qed.
-
-  Instance lt_strorder : StrictOrder lt := {
-    StrictOrder_Irreflexive := lt_irreflexive ;
-    StrictOrder_Transitive := lt_transitive
-  }.
-
-  Instance lt_compat : Proper (eq ==> eq ==> iff) lt.
-  Proof. solve_proper. Qed.
-
-  Lemma compare_spec : forall x y : Var, CompareSpec (x = y) (lt x y) (lt y x) (compare x y).
-  Proof.
-    intros x y. destruct (compare x y) eqn:Hxy; destruct x; destruct y;
-      simpl in Hxy; constructor; first
-        [ apply NF.compare_eq_iff in Hxy
-        | apply NF.compare_lt_iff in Hxy
-        | apply NF.compare_gt_iff in Hxy
-        ]; auto.
-  Qed.
-
-End VarOrder.
+End VarEq.
